Especificaciones/VertexCoverOpt.dfy
@@ -40,6 +40,7 @@ ghost predicate optimalVertexCover (graph: Graph, I : set<Node>)
     && forall S: set<Node> | S <= graph.0 && isVertexCover(S, graph) :: |S| >= |I|
 }
 
+
 lemma boundoptimalVertexCover(graph: Graph, I : set<Node>) 
 requires isValidGraph(graph)
 requires optimalVertexCover(graph,I)
